With some likely true lemmas about memory preservation, we can prove that the top-level procedure computes poly1305!

src/crypto/poly1305/x64/X64.Poly1305.Math_i.fst
@@ -21,6 +21,12 @@ lemma_BitwiseMul64()
 
 // #reset-options "--z3rlimit 1200 --z3cliopt smt.QI.EAGER_THRESHOLD=100 --z3cliopt smt.CASE_SPLIT=3 --z3cliopt smt.arith.nl=false --max_fuel 0 --max_ifuel 0 --smtencoding.elim_box true --eager_inference --smtencoding.nl_arith_repr wrapped --smtencoding.l_arith_repr native"
 
+let heapletTo128_preserved (m:mem) (m':mem) (i:int) (len:nat) =
+  admit()
+
+let heapletTo128_all_preserved (m:mem)(i:int) (len:nat) =
+  admit()
+
 let rec poly1305_heap_blocks (h:int) (pad:int) (r:int) (m:mem) (i:int) 
         (k:int{i <= k /\ (k - i) % 16 == 0 /\ (forall (j:int) . {:pattern (m `Map.contains` j)} i <= j /\ j < k /\ (j - i) % 8 = 0 ==> m `Map.contains` j)}) : Tot int (decreases (k - i)) =
         admit()
